$$
\begin{align}
f(x) &= cx^{n} \\
f(x)'&= cn \ast x^{n -1}
\end{align}
$$

$$
(f \circ g)'(x) = f'\big( g(x) \big ) g'(x)
$$





$$
\mathcal{L} = \frac{1}{2} (y - t) ^ 2
$$

令：$z = y - t$,  则  $\mathcal{L} = \frac{1}{2} z ^ 2 \\$,  根据链式法则有：

 $\frac{\partial \mathcal{L}}{\partial z} = \frac{1}{2} * 2 * z = z$ ,  $\frac{\partial \mathcal{z}}{\partial y} = 1$

$\frac{\partial \mathcal{L}}{\partial y} = \frac{\partial \mathcal{L}}{\partial z} \frac{\partial \mathcal{z}}{\partial y} = z * 1 = z = y - t$   



根据复合函数求导法则： $(f \circ g)'(x) = f'\big( g(x) \big ) g'(x)$ 有，



$$
(\mathcal{L} \circ z)'(y) = \mathcal{L}' ( z(y) ) z'(y) \\
= z(z(y)) \\
= z(y-t) \\
= (y-t) -t \\
= y - 2t
$$








